Big update of semantics to support internal calls
The steps are a lot smaller now, with explicit continuations
representing all the contexts a call might return to.

An alternative approach (which maybe we will want to prove equivalent at
some point?) would be to make statement and expression semantics
mutually recursive, leaving the continuations implicit.

The test theorems are not updated yet (except for one). Execution by
rewriting is a lot slower now so possibly we want to cv_translate the
semantics for execution.

vyperVmScript.sml
@@ -16,44 +16,21 @@ Datatype:
   | StructV ((identifier, value) alist)
 End
 
-Definition evaluate_literal_def:
-  evaluate_literal (BoolL b)   = BoolV b ∧
-  evaluate_literal (StringL s) = StringV s ∧
-  evaluate_literal (BytesL bs) = BytesV bs ∧
-  evaluate_literal (IntL i)    = IntV i
-End
-
 Datatype:
-  expr_result = Err | Vs (value list)
+  toplevel_value = Value value | HashMap ((value, toplevel_value) alist)
 End
 
-Definition evaluate_cmp_def:
-  evaluate_cmp Eq    (StringV s1) (StringV s2) = Vs [BoolV (s1 = s2)] ∧
-  evaluate_cmp Eq    (IntV i1)    (IntV i2)    = Vs [BoolV (i1 = i2)] ∧
-  evaluate_cmp NotEq (StringV s1) (StringV s2) = Vs [BoolV (s1 ≠ s2)] ∧
-  evaluate_cmp NotEq (IntV i1)    (IntV i2)    = Vs [BoolV (i1 ≠ i2)] ∧
-  evaluate_cmp _ _ _ = Err
-End
-
-Definition evaluate_binop_def:
-  evaluate_binop Add (IntV i1) (IntV i2) = Vs [IntV (i1 + i2)] ∧
-  evaluate_binop Sub (IntV i1) (IntV i2) = Vs [IntV (i1 - i2)] ∧
-  evaluate_binop (_: operator) _ _ = Err
-End
-
-Definition expr_nodes_def:
-  expr_nodes (NamedExpr e1 e2) = 1n + expr_nodes e1 + expr_nodes e2 ∧
-  expr_nodes (Name _) = 1 + 1 ∧
-  expr_nodes (GlobalName _) = 1 + 1 ∧
-  expr_nodes (IfExp e1 e2 e3) = 1 + expr_nodes e1 + expr_nodes e2 + expr_nodes e3 ∧
-  expr_nodes (Literal _) = 1 + 1 ∧
-  expr_nodes (ArrayLit es) = 1 + LENGTH es + SUM (MAP expr_nodes es) ∧
-  expr_nodes (Compare e1 _ e2) = 1 + expr_nodes e1 + 1 + expr_nodes e2 ∧
-  expr_nodes (BinOp e1 _ e2) = 1 + expr_nodes e1 + 1 + expr_nodes e2 ∧
-  expr_nodes (Subscript e1 e2) = 1 + 2 + expr_nodes e1 + expr_nodes e2 ∧
-  expr_nodes (Attribute e _) = 1 + expr_nodes e + 1
+Definition default_value_def:
+  default_value (BaseT (UintT _)) = IntV 0 ∧
+  default_value (BaseT (IntT _)) = IntV 0 ∧
+  default_value (TupleT ts) = TupleV (MAP default_value ts) ∧
+  default_value (DynArrayT _ _) = ArrayV [] ∧
+  default_value VoidT = VoidV ∧
+  default_value (BaseT BoolT) = BoolV F ∧
+  default_value (BaseT StringT) = StringV "" ∧
+  default_value (BaseT BytesT) = BytesV []
 Termination
-  WF_REL_TAC`measure expr_size`
+  WF_REL_TAC ‘measure type_size’
 End
 
 Type scope = “:identifier |-> value”;
@@ -64,6 +41,114 @@ Definition lookup_scopes_def:
   case FLOOKUP env id of NONE =>
     lookup_scopes id rest
   | SOME v => SOME v
+End
+
+Datatype:
+  expr_continuation
+  = StartExpr expr
+  (*
+  | NamedExprK1 expr_continuation expr
+  | NamedExprK2 value expr_continuation
+  *)
+  | IfExpK expr_continuation expr expr
+  | ArrayLitK (value list) expr_continuation (expr list)
+  | SubscriptK1 expr_continuation expr
+  | SubscriptK2 value expr_continuation
+  | AttributeK expr_continuation identifier
+  | CompareK1 expr_continuation cmpop expr
+  | CompareK2 value cmpop expr_continuation
+  | BinOpK1 expr_continuation operator expr
+  | BinOpK2 value operator expr_continuation
+  | CallK identifier (value list) expr_continuation (expr list)
+  | LiftCall identifier (value list) expr_continuation
+  | DoneExpr value
+  | ReturnExpr
+  | ErrorExpr
+End
+
+Type containing_scope = “: scope list # scope # scope list”;
+
+Datatype:
+  location
+  = ScopedVar containing_scope identifier
+  | Global identifier
+End
+
+Datatype:
+  subscript
+  = IntSubscript int
+  | StrSubscript string
+  | AttrSubscript identifier
+End
+
+Datatype:
+  assignment_value
+  = BaseTargetV location (subscript list)
+  | TupleTargetV (assignment_value list)
+End
+
+Datatype:
+  base_tgt_continuation
+  = StartBaseTgt base_assignment_target
+  | SubscriptTargetK1 base_tgt_continuation expr
+  | SubscriptTargetK2 location (subscript list) expr_continuation
+  | AttributeTargetK base_tgt_continuation identifier
+  | LiftCallBaseTgt identifier (value list) base_tgt_continuation
+  | DoneBaseTgt location (subscript list)
+End
+
+Datatype:
+  tgt_continuation
+  = StartTgt assignment_target
+  | TupleTargetK (assignment_value list) tgt_continuation (assignment_target list)
+  | BaseTargetK base_tgt_continuation
+  | LiftCallTgt identifier (value list) tgt_continuation
+  | DoneTgt assignment_value
+  | ErrorTgt
+End
+
+Datatype:
+  exception
+  = RaiseException string
+  | AssertException string
+  | Error
+  | ExternalReturn value
+End
+
+Datatype:
+  stmt_continuation
+  = StartK stmt
+  | IfK expr_continuation (stmt list) (stmt list)
+  | AssertK expr_continuation string
+  | ReturnSomeK expr_continuation
+  | AssignK1 tgt_continuation expr
+  | AssignK2 assignment_value expr_continuation
+  | AugAssignK identifier operator expr_continuation
+  | AnnAssignK identifier type expr_continuation
+  | ForK identifier type expr_continuation (stmt list)
+  | DoneK
+  | ExceptionK exception
+End
+
+Definition evaluate_literal_def:
+  evaluate_literal (BoolL b)   = BoolV b ∧
+  evaluate_literal (StringL s) = StringV s ∧
+  evaluate_literal (BytesL bs) = BytesV bs ∧
+  evaluate_literal (IntL i)    = IntV i
+End
+
+Definition evaluate_cmp_def:
+  evaluate_cmp Eq    (StringV s1) (StringV s2) = DoneExpr (BoolV (s1 = s2)) ∧
+  evaluate_cmp Eq    (IntV i1)    (IntV i2)    = DoneExpr (BoolV (i1 = i2)) ∧
+  evaluate_cmp NotEq (StringV s1) (StringV s2) = DoneExpr (BoolV (s1 ≠ s2)) ∧
+  evaluate_cmp NotEq (IntV i1)    (IntV i2)    = DoneExpr (BoolV (i1 ≠ i2)) ∧
+  evaluate_cmp _ _ _ = ErrorExpr
+End
+
+Definition evaluate_binop_def:
+  evaluate_binop Add (IntV i1) (IntV i2) = DoneExpr (IntV (i1 + i2)) ∧
+  evaluate_binop Sub (IntV i1) (IntV i2) = DoneExpr (IntV (i1 - i2)) ∧
+  evaluate_binop (_: operator) _ _ = ErrorExpr
 End
 
 Definition extract_elements_def:
@@ -85,139 +170,217 @@ Definition integer_index_def:
    else NONE
 End
 
+Definition evaluate_subscript_def:
+  evaluate_subscript av (IntV i) =
+  (case extract_elements av of SOME vs =>
+    (case integer_index vs i of SOME j => DoneExpr (EL j vs)
+     | _ => ErrorExpr)
+   | _ => ErrorExpr) ∧
+  evaluate_subscript _ _ = ErrorExpr
+End
+
+Definition evaluate_attribute_def:
+  evaluate_attribute (StructV kvs) id =
+  (case ALOOKUP kvs id of SOME v => DoneExpr v
+   | _ => ErrorExpr) ∧
+  evaluate_attribute _ _ = ErrorExpr
+End
+
+Definition step_expr_def:
+  step_expr gbs env (StartExpr (Literal l)) =
+    DoneExpr (evaluate_literal l) ∧
+  step_expr gbs env (StartExpr (ArrayLit [])) =
+    DoneExpr (ArrayV []) ∧
+  step_expr gbs env (StartExpr (ArrayLit (e::es))) =
+    ArrayLitK [] (StartExpr e) es ∧
+  step_expr gbs env (StartExpr (Name id)) =
+    (case lookup_scopes id env
+     of SOME v => DoneExpr v
+      | _ => ErrorExpr) ∧
+  step_expr gbs env (StartExpr (GlobalName id)) =
+    (case FLOOKUP gbs id
+     of SOME (Value v) => DoneExpr v
+      | _ => ErrorExpr) ∧
+  step_expr gbs env (StartExpr (Subscript e1 e2)) =
+    SubscriptK1 (StartExpr e1) e2 ∧
+  step_expr gbs env (StartExpr (Attribute e id)) =
+    AttributeK (StartExpr e) id ∧
+  step_expr gbs env (StartExpr (IfExp e1 e2 e3)) =
+    IfExpK (StartExpr e1) e2 e3 ∧
+  step_expr gbs env (StartExpr (Compare e1 cmp e2)) =
+    CompareK1 (StartExpr e1) cmp e2 ∧
+  step_expr gbs env (StartExpr (BinOp e1 bop e2)) =
+    BinOpK1 (StartExpr e1) bop e2 ∧
+  step_expr gbs env (StartExpr (Call id [])) =
+    LiftCall id [] ReturnExpr ∧
+  step_expr gbs env (StartExpr (Call id (e::es))) =
+    CallK id [] (StartExpr e) es ∧
+  (*
+  step_expr gbs env (NamedExprK1 k e) =
+    (case step_expr gbs env k
+     of ErrorExpr => ErrorExpr
+      | DoneExpr v => NamedExprK2 v (StartExpr e)
+      | LiftCall id vs k => LiftCall id vs (NamedExprK1 k e)
+      | k => NamedExprK1 k e) ∧
+  step_expr gbs env (NamedExprK2 v1 k) =
+    (case step_expr gbs env k
+     of ErrorExpr => ErrorExpr
+      | DoneExpr v2 =>
+  *)
+  step_expr gbs env (IfExpK k e2 e3) =
+  (case step_expr gbs env k
+   of ErrorExpr => ErrorExpr
+    | DoneExpr v1 => (case v1 of BoolV b => StartExpr (if b then e2 else e3)
+                               | _ => ErrorExpr)
+    | LiftCall id vs k => LiftCall id vs (IfExpK k e2 e3)
+    | k => IfExpK k e2 e3) ∧
+  step_expr gbs env (ArrayLitK vs k es) =
+  (case step_expr gbs env k
+   of ErrorExpr => ErrorExpr
+    | DoneExpr v =>
+        (case es of (e::es) => ArrayLitK (SNOC v vs) (StartExpr e) es
+                  | [] => DoneExpr (ArrayV (SNOC v vs)))
+    | LiftCall id as k => LiftCall id as (ArrayLitK vs k es)
+    | k => ArrayLitK vs k es) ∧
+  step_expr gbs env (SubscriptK1 k e) =
+  (case step_expr gbs env k
+   of ErrorExpr => ErrorExpr
+    | DoneExpr v => SubscriptK2 v (StartExpr e)
+    | LiftCall id vs k => LiftCall id vs (SubscriptK1 k e)
+    | k => SubscriptK1 k e) ∧
+  step_expr gbs env (SubscriptK2 v1 k) =
+  (case step_expr gbs env k
+   of ErrorExpr => ErrorExpr
+    | DoneExpr v2 => evaluate_subscript v1 v2
+    | LiftCall id vs k => LiftCall id vs (SubscriptK2 v1 k)
+    | k => SubscriptK2 v1 k) ∧
+  step_expr gbs env (AttributeK k id) =
+  (case step_expr gbs env k
+   of ErrorExpr => ErrorExpr
+    | DoneExpr v => evaluate_attribute v id
+    | LiftCall id vs k => LiftCall id vs (AttributeK k id)
+    | k => AttributeK k id) ∧
+  step_expr gbs env (CompareK1 k cmp e2) =
+  (case step_expr gbs env k
+   of ErrorExpr => ErrorExpr
+    | DoneExpr v1 => CompareK2 v1 cmp (StartExpr e2)
+    | LiftCall id vs k => LiftCall id vs (CompareK1 k cmp e2)
+    | k => CompareK1 k cmp e2) ∧
+  step_expr gbs env (CompareK2 v1 cmp k) =
+  (case step_expr gbs env k
+   of ErrorExpr => ErrorExpr
+    | DoneExpr v2 => evaluate_cmp cmp v1 v2
+    | LiftCall id vs k => LiftCall id vs (CompareK2 v1 cmp k)
+    | k => CompareK2 v1 cmp k) ∧
+  step_expr gbs env (BinOpK1 k bop e2) =
+  (case step_expr gbs env k
+   of ErrorExpr => ErrorExpr
+    | DoneExpr v1 => BinOpK2 v1 bop (StartExpr e2)
+    | LiftCall id vs k => LiftCall id vs (BinOpK1 k bop e2)
+    | k => BinOpK1 k bop e2) ∧
+  step_expr gbs env (BinOpK2 v1 bop k) =
+  (case step_expr gbs env k
+   of ErrorExpr => ErrorExpr
+    | DoneExpr v2 => evaluate_binop bop v1 v2
+    | LiftCall id vs k => LiftCall id vs (BinOpK2 v1 bop k)
+    | k => BinOpK2 v1 bop k) ∧
+  step_expr gbs env (CallK id vs k es) =
+  (case step_expr gbs env k
+   of ErrorExpr => ErrorExpr
+    | DoneExpr v =>
+        (case es of (e::es) => CallK id (SNOC v vs) (StartExpr e) es
+                  | [] => LiftCall id (SNOC v vs) ReturnExpr)
+    | LiftCall id vs k => LiftCall id vs (CallK id vs k es)
+    | k => CallK id vs k es) ∧
+  step_expr gbs env (LiftCall id vs k) = LiftCall id vs k ∧
+  step_expr gbs env (DoneExpr v) = DoneExpr v ∧
+  step_expr gbs env ReturnExpr = ReturnExpr ∧
+  step_expr gbs env ErrorExpr = ErrorExpr
+End
+
 Datatype:
-  toplevel_value = Value value | HashMap ((value, toplevel_value) alist)
-End
-
-Definition evaluate_exps_def:
-  evaluate_exps gbs env [Literal l] = Vs [evaluate_literal l] ∧
-  evaluate_exps gbs env [ArrayLit es] =
-  (case evaluate_exps gbs env es of
-        Vs vs => Vs [ArrayV vs]
-      | _ => Err) ∧
-  evaluate_exps gbs env [Name id] =
-  (case lookup_scopes id env of SOME v => Vs [v]
-   | _ => Err) ∧
-  evaluate_exps gbs env [GlobalName id] =
-  (case FLOOKUP gbs id of SOME (Value v) => Vs [v] | _ => Err) ∧
-  evaluate_exps gbs env [Subscript e1 e2] =
-  (case evaluate_exps gbs env [e1; e2] of Vs [av; IntV i] =>
-   (case extract_elements av of SOME vs =>
-    (case integer_index vs i of SOME j => Vs [EL j vs]
-     | _ => Err) | _ => Err) | _ => Err) ∧
-  evaluate_exps gbs env [Attribute e id] =
-  (case evaluate_exps gbs env [e] of Vs [StructV kvs] =>
-   (case ALOOKUP kvs id of SOME v => Vs [v]
-       | _ => Err) | _ => Err) ∧
-  evaluate_exps gbs env [IfExp e1 e2 e3] =
-  (case evaluate_exps gbs env [e1] of Vs [BoolV b] =>
-     if b then evaluate_exps gbs env [e2] else evaluate_exps gbs env [e3]
-   | _ => Err) ∧
-  evaluate_exps gbs env [Compare e1 cmp e2] =
-  (case evaluate_exps gbs env [e1; e2] of Vs [v1; v2] =>
-     evaluate_cmp cmp v1 v2
-   | _ => Err) ∧
-  evaluate_exps gbs env [BinOp e1 bop e2] =
-  (case evaluate_exps gbs env [e1; e2] of Vs [v1; v2] =>
-     evaluate_binop bop v1 v2
-   | _ => Err) ∧
-  evaluate_exps gbs env [] = Vs [] ∧
-  evaluate_exps gbs env [e1] = Err ∧
-  evaluate_exps gbs env (e1::es) =
-  (case evaluate_exps gbs env [e1] of Vs [v1] =>
-    (case evaluate_exps gbs env es of Vs vs => Vs (v1::vs) | x => x)
-   | x => x)
-Termination
-  WF_REL_TAC`measure ((λls. LENGTH ls + SUM (MAP expr_nodes ls)) o SND o SND)`
-  \\ rw[expr_nodes_def, ETA_AX]
-End
-
-Definition default_value_def:
-  default_value (BaseT (UintT _)) = IntV 0 ∧
-  default_value (BaseT (IntT _)) = IntV 0 ∧
-  default_value (TupleT ts) = TupleV (MAP default_value ts) ∧
-  default_value (DynArrayT _ _) = ArrayV [] ∧
-  default_value VoidT = VoidV ∧
-  default_value (BaseT BoolT) = BoolV F ∧
-  default_value (BaseT StringT) = StringV "" ∧
-  default_value (BaseT BytesT) = BytesV []
-Termination
-  WF_REL_TAC ‘measure type_size’
-End
-
-Datatype:
-  exception
-  = BreakException
-  | ContinueException
-  | ReturnException value
-  | RaiseException string
-  | AssertException string
-  | Error
-  | Timeout
-End
-
-Datatype:
-  function_context = <|
-    scopes: scope list
-  ; return_to: expr option (* TODO *)
-  ; continuation: stmt list
+  loop_info = <|
+    loop_var: identifier
+  ; loop_first_stmt: stmt
+  ; loop_rest_stmts: stmt list
+  ; remaining_values: value list
   |>
+End
+
+Datatype:
+  function_context =
+  <| scopes: scope list
+   ; current_stmt: stmt_continuation
+   ; remaining_stmts: stmt list
+   ; loop: loop_info option
+   |>
 End
 
 Datatype:
   execution_context = <|
-    call_stack: function_context list
+    current_fc : function_context
+  ; call_stack : function_context list
   ; globals: identifier |-> toplevel_value
-  ; raised: exception option
+  ; contract: toplevel list
   |>
 End
 
 Definition initial_function_context_def:
-  initial_function_context args body = <|
+  initial_function_context args ss = <|
     scopes := [args]
-  ; return_to := NONE
-  ; continuation := body
+  ; current_stmt := (case ss of s::_ => StartK s | _ => ExceptionK Error)
+  ; remaining_stmts := TL ss
+  ; loop := NONE
   |>
 End
 
+(* TODO: assumes unique identifiers, but should check? *)
+Definition initial_globals_def:
+  initial_globals [] = FEMPTY ∧
+  initial_globals (VariableDecl id typ _ Storage :: ts) =
+  initial_globals ts |+ (id, Value $ default_value typ) ∧
+  initial_globals (VariableDecl id typ _ Transient :: ts) =
+  initial_globals ts |+ (id, Value $ default_value typ) ∧
+  (* TODO: handle Constants and  Immutables *)
+  initial_globals (t :: ts) = initial_globals ts
+  (* TODO: hashmap toplevels *)
+End
+
 Definition initial_execution_context_def:
-  initial_execution_context gbs fc = <|
-    call_stack := [fc]
-  ; globals := gbs
-  ; raised := NONE
+  initial_execution_context ts fc = <|
+    current_fc := fc
+  ; call_stack := []
+  ; globals := initial_globals ts
+  ; contract := ts
   |>
 End
 
 Definition raise_def:
-  raise err ctx = ctx with raised := SOME err
+  raise err ctx = ctx with current_fc updated_by
+    (λfc. fc with current_stmt := ExceptionK err)
 End
 
 Definition push_scope_def:
   push_scope ctx =
-  case ctx.call_stack of fc::rest =>
-    ctx with call_stack := (fc with scopes updated_by CONS FEMPTY) :: rest
-  | _ => raise Error ctx
+    ctx with current_fc updated_by (λfc. fc with scopes updated_by CONS FEMPTY)
 End
 
 Definition pop_scope_def:
   pop_scope ctx =
-  case ctx.call_stack of fc::fcs =>
-    (case fc.scopes of [] => raise Error ctx
-     | (_::rest) => ctx with call_stack := (fc with scopes := rest)::fcs)
-  | _ => raise Error ctx
+  case ctx.current_fc.scopes
+    of [] => raise Error ctx
+     | (_::rest) => ctx with current_fc updated_by (λfc. fc with scopes := rest)
 End
 
 Definition new_variable_def:
   new_variable id typ ctx =
-  case ctx.call_stack of fc::fcs =>
-    (case fc.scopes of [] => raise Error ctx
-     | env::rest => if id ∈ FDOM env then raise Error ctx else
-       ctx with call_stack :=
-         (fc with scopes := (env |+ (id, default_value typ))::rest)::fcs)
-  | _ => raise Error ctx
+  case ctx.current_fc.scopes
+    of [] => raise Error ctx
+     | env::rest =>
+         if id ∈ FDOM env then raise Error ctx
+         else ctx with current_fc updated_by
+           (λfc. fc with scopes := (env |+ (id, default_value typ))::rest)
 End
-
-Type containing_scope = “: scope list # scope # scope list”;
 
 Definition find_containing_scope_def:
   find_containing_scope id [] = NONE : containing_scope option ∧
@@ -226,63 +389,78 @@ Definition find_containing_scope_def:
   else OPTION_MAP (λ(p,q). (env::p, q)) (find_containing_scope id rest)
 End
 
-Datatype:
-  location
-  = ScopedVar containing_scope identifier
-  | Global identifier
+Definition step_base_target_def:
+  step_base_target gbs env (StartBaseTgt (NameTarget id)) =
+    (case find_containing_scope id env
+     of SOME cs => SOME $ DoneBaseTgt (ScopedVar cs id) []
+      | _ => NONE) ∧
+  step_base_target gbs env (StartBaseTgt (GlobalNameTarget id)) =
+    SOME $ DoneBaseTgt (Global id) [] ∧
+  step_base_target gbs env (StartBaseTgt (SubscriptTarget t e)) =
+  SOME $ SubscriptTargetK1 (StartBaseTgt t) e ∧
+  step_base_target gbs env (StartBaseTgt (AttributeTarget t id)) =
+  SOME $ AttributeTargetK (StartBaseTgt t) id ∧
+  step_base_target gbs env (SubscriptTargetK1 k e) =
+    (case step_base_target gbs env k of
+     | SOME (DoneBaseTgt l s) =>
+         SOME $ SubscriptTargetK2 l s (StartExpr e)
+     | SOME (LiftCallBaseTgt fn vs k) =>
+         SOME $ LiftCallBaseTgt fn vs (SubscriptTargetK1 k e)
+     | SOME k => SOME $ SubscriptTargetK1 k e
+     | _ => NONE) ∧
+  step_base_target gbs env (SubscriptTargetK2 l s k) =
+   (case step_expr gbs env k
+    of DoneExpr (IntV i) => SOME $ DoneBaseTgt l ((IntSubscript i)::s)
+     | DoneExpr _ => NONE
+     | ErrorExpr => NONE
+     | LiftCall fn vs k => SOME $ LiftCallBaseTgt fn vs (SubscriptTargetK2 l s k)
+     | k => SOME $ SubscriptTargetK2 l s k) ∧
+  step_base_target gbs env (AttributeTargetK k id) =
+  (case step_base_target gbs env k
+   of NONE => NONE
+    | SOME (DoneBaseTgt l s) =>
+        SOME $ DoneBaseTgt l ((AttrSubscript id)::s)
+    | SOME (LiftCallBaseTgt fn vs k) =>
+        SOME $ LiftCallBaseTgt fn vs (AttributeTargetK k id)
+    | SOME k => SOME $ AttributeTargetK k id
+    | _ => NONE)
 End
 
-Datatype:
-  subscript
-  = IntSubscript int
-  | StrSubscript string
-  | AttrSubscript identifier
-End
-
-Datatype:
-  assignment_value
-  = BaseTargetV location (subscript list)
-  | TupleTargetV (assignment_value list)
-End
-
-Definition add_subscript_def:
-  add_subscript (l: location, ls) (i: subscript) = (l, i::ls)
-End
-
-Definition evaluate_base_target_def:
-  evaluate_base_target gbs env (NameTarget id) =
-    OPTION_MAP (λcs. (ScopedVar cs id,[])) (find_containing_scope id env) ∧
-  evaluate_base_target gbs env (GlobalNameTarget id) = SOME $ (Global id, []) ∧
-  evaluate_base_target gbs env (SubscriptTarget t e) =
-  (case evaluate_base_target gbs env t of NONE => NONE | SOME v =>
-   (case evaluate_exps gbs env [e] of Vs [IntV i] =>
-      SOME $ add_subscript v (IntSubscript i)
-    | _ => NONE)) ∧
-  evaluate_base_target gbs env (AttributeTarget t id) =
-  (case evaluate_base_target gbs env t of NONE => NONE | SOME v =>
-   SOME $ add_subscript v (AttrSubscript id))
-End
-
-Definition evaluate_target_def:
-  evaluate_target gbs env (BaseTarget b) =
-  OPTION_MAP (UNCURRY BaseTargetV) (evaluate_base_target gbs env b) ∧
-  evaluate_target gbs env (TupleTarget []) = SOME $ TupleTargetV [] ∧
-  evaluate_target gbs env (TupleTarget (t::ts)) =
-  (case evaluate_target gbs env t of NONE => NONE | SOME v =>
-   case evaluate_target gbs env (TupleTarget ts) of SOME (TupleTargetV vs) =>
-     SOME (TupleTargetV (v::vs)) | _ => NONE)
+Definition step_target_def:
+  step_target gbs env (StartTgt (BaseTarget b)) =
+    BaseTargetK (StartBaseTgt b) ∧
+  step_target gbs env (StartTgt (TupleTarget [])) =
+    DoneTgt (TupleTargetV []) ∧
+  step_target gbs env (StartTgt (TupleTarget (t::ts))) =
+    TupleTargetK [] (StartTgt t) ts ∧
+  step_target gbs env (TupleTargetK vs k ts) =
+  (case step_target gbs env k
+   of DoneTgt v =>
+     (case ts of [] => DoneTgt (TupleTargetV (SNOC v vs))
+               | (t::ts) => TupleTargetK (SNOC v vs) (StartTgt t) ts)
+    | LiftCallTgt fn as k =>
+        LiftCallTgt fn as (TupleTargetK vs k ts)
+    | ErrorTgt => ErrorTgt
+    | k => TupleTargetK vs k ts) ∧
+  step_target gbs env (BaseTargetK k) =
+  (case step_base_target gbs env k
+   of SOME (DoneBaseTgt l s) => DoneTgt $ BaseTargetV l s
+    | SOME (LiftCallBaseTgt fn vs k) => LiftCallTgt fn vs (BaseTargetK k)
+    | SOME k => BaseTargetK k
+    | _ => ErrorTgt) ∧
+  step_target gbs env (LiftCallTgt fn vs k) = LiftCallTgt fn vs k ∧
+  step_target gbs env (DoneTgt v) = DoneTgt v ∧
+  step_target gbs env _ = ErrorTgt
 End
 
 Definition set_variable_def:
   set_variable id v ctx =
-  case ctx.call_stack of fc::fcs =>
-    (case find_containing_scope id fc.scopes of
-       NONE => raise Error ctx
+  case find_containing_scope id ctx.current_fc.scopes
+    of NONE => raise Error ctx
      | SOME (pre, env, rest) =>
-       (* check that v has same type as current value here ? *)
-       ctx with call_stack :=
-         (fc with scopes := pre ++ (env |+ (id, v))::rest)::fcs)
-  | _ => raise Error ctx
+         (* check that v has same type as current value here ? *)
+         ctx with current_fc updated_by
+           (λfc. fc with scopes := pre ++ (env |+ (id, v))::rest)
 End
 
 Definition assign_subscripts_def:
@@ -300,14 +478,12 @@ End
 
 Definition assign_target_def:
   assign_target (BaseTargetV (ScopedVar (pre,env,rest) id) is) v ctx =
-  (case ctx.call_stack of fc::fcs =>
     (case FLOOKUP env id of SOME a =>
      (case assign_subscripts a is v of SOME a' =>
-        ctx with call_stack :=
-          (fc with scopes := pre ++ (env |+ (id, a'))::rest)::fcs
+        ctx with current_fc updated_by
+          (λfc. fc with scopes := pre ++ (env |+ (id, a'))::rest)
       | _ => raise Error ctx)
-     | _ => raise Error ctx)
-   | _ => raise Error ctx) ∧
+     | _ => raise Error ctx) ∧
   assign_target (BaseTargetV (Global id) is) v ctx =
   (* TODO: add assignment to hashmaps *)
   (case FLOOKUP ctx.globals id of SOME (Value a) =>
@@ -318,102 +494,12 @@ Definition assign_target_def:
   assign_target _ _ ctx = raise Error ctx (* TODO: handle TupleTargetV *)
 End
 
-(* TODO: remove clock:
-* - ensure For statement bound (DynArray max size, or range max) is present on syntax
-* - define bound on execution steps for statements syntactically
-* - use that to craft the termination measure *)
-
-(* TODO: use state-exception monad *)
-
-Definition execute_stmts_def:
-  execute_stmts n [Pass] ctx = ctx ∧
-  execute_stmts n [Continue] ctx = raise ContinueException ctx ∧
-  execute_stmts n [Break] ctx = raise BreakException ctx ∧
-  execute_stmts n [Raise s] ctx = raise (RaiseException s) ctx ∧
-  execute_stmts n [Return NONE] ctx = raise (ReturnException VoidV) ctx ∧
-  execute_stmts n [Return (SOME e)] ctx =
-  (case ctx.call_stack of fc::_ =>
-   (case evaluate_exps ctx.globals fc.scopes [e] of Vs [v] =>
-     raise (ReturnException v) ctx
-    | _ => raise Error ctx)
-   | _ => raise Error ctx) ∧
-  execute_stmts n [AnnAssign id typ e] ctx =
-  (let ctx = new_variable id typ ctx in
-   if IS_SOME ctx.raised then ctx else
-   (case ctx.call_stack of fc::_ =>
-     (case evaluate_exps ctx.globals fc.scopes [e] of Vs [v] =>
-        set_variable id v ctx
-      | _ => raise Error ctx)
-    | _ => raise Error ctx)) ∧
-  execute_stmts n [AugAssign id bop e2] ctx =
-  (case ctx.call_stack of fc::_ =>
-    (case lookup_scopes id fc.scopes of NONE => raise Error ctx | SOME v1 =>
-     case evaluate_exps ctx.globals fc.scopes [e2] of Vs [v2] =>
-     (case evaluate_binop bop v1 v2 of Vs [v] =>
-        set_variable id v ctx
-      | _ => raise Error ctx)
-     | _ => raise Error ctx)
-   | _ => raise Error ctx) ∧
-  execute_stmts n [Assign tgt e] ctx =
-   (case ctx.call_stack of fc::_ =>
-     (case evaluate_exps ctx.globals fc.scopes [e] of Vs [v] =>
-      (case evaluate_target ctx.globals fc.scopes tgt of SOME tv =>
-        assign_target tv v ctx
-       | _ => raise Error ctx)
-      | _ => raise Error ctx)
-    | _ => raise Error ctx) ∧
-  execute_stmts n [If e s1 s2] ctx =
-  (if n = 0 then raise Timeout ctx else
-   (case ctx.call_stack of fc::_ =>
-     (case evaluate_exps ctx.globals fc.scopes [e] of Vs [BoolV b] =>
-       execute_stmts (PRE n) (if b then s1 else s2) ctx
-      | _ => raise Error ctx)
-   | _ => raise Error ctx)) ∧
-  execute_stmts n [For id typ e ss] ctx =
-  (case ctx.call_stack of fc::_ =>
-    (case evaluate_exps ctx.globals fc.scopes [e] of Vs [ArrayV vs] =>
-     let
-       ctx = push_scope ctx;
-       ctx = new_variable id typ ctx;
-     in
-       if IS_SOME ctx.raised then ctx else
-       if n = 0 then raise Timeout ctx else
-         execute_for (PRE n) id typ ss vs ctx
-     | _ => raise Error ctx)
-   | _ => raise Error ctx) ∧
-  execute_stmts n [_] ctx = raise Error ctx ∧
-  execute_stmts n [] ctx = ctx ∧
-  execute_stmts n (s1::ss) ctx =
-  (if n = 0 then raise Timeout ctx else
-    let ctx = execute_stmts (PRE n) [s1] ctx in
-      if IS_SOME ctx.raised then ctx else
-      execute_stmts (PRE n) ss ctx) ∧
-  execute_for n id typ ss [] ctx = pop_scope ctx ∧
-  execute_for n id typ ss (v::vs) ctx =
-  (let ctx = push_scope ctx in
-   let ctx = set_variable id v ctx in
-    if IS_SOME ctx.raised then ctx else
-    if n = 0 then raise Timeout ctx else
-   let ctx = execute_stmts (PRE n) ss ctx in
-    if IS_SOME ctx.raised then ctx else
-   let ctx = pop_scope ctx in
-    if IS_SOME ctx.raised then ctx else
-   execute_for (PRE n) id typ ss vs ctx)
-Termination
-  WF_REL_TAC`measure (λx. case x of
-    (INR (n,_) => n) | (INL (n,_) => n))`
-End
-
-(* TODO: assumes unique identifiers, but should check? *)
-Definition initial_globals_def:
-  initial_globals [] = FEMPTY ∧
-  initial_globals (VariableDecl id typ _ Storage :: ts) =
-  initial_globals ts |+ (id, Value $ default_value typ) ∧
-  initial_globals (VariableDecl id typ _ Transient :: ts) =
-  initial_globals ts |+ (id, Value $ default_value typ) ∧
-  (* TODO: handle Constants and  Immutables *)
-  initial_globals (t :: ts) = initial_globals ts
-  (* TODO: hashmap toplevels *)
+(* TODO: check types? *)
+Definition bind_arguments_def:
+  bind_arguments ([]: argument list) [] = SOME (FEMPTY: scope) ∧
+  bind_arguments ((id, typ)::params) (v::vs) =
+    OPTION_MAP (λm. m |+ (id, v)) (bind_arguments params vs) ∧
+  bind_arguments _ _ = NONE
 End
 
 Definition lookup_external_function_def:
@@ -425,27 +511,305 @@ Definition lookup_external_function_def:
     lookup_external_function name ts
 End
 
-(* TODO: check types? *)
-Definition bind_arguments_def:
-  bind_arguments ([]: argument list) [] = SOME (FEMPTY: scope) ∧
-  bind_arguments ((id, typ)::params) (v::vs) =
-    OPTION_MAP (λm. m |+ (id, v)) (bind_arguments params vs) ∧
-  bind_arguments _ _ = NONE
+Definition push_call_def:
+  push_call fn args ctx =
+  case lookup_external_function fn ctx.contract of
+  | SOME (params, ret, body) =>
+    (case bind_arguments params args of
+     | SOME env =>
+         let fc = initial_function_context env body in
+         ctx with <|
+           call_stack updated_by CONS ctx.current_fc
+         ; current_fc := fc |>
+     | _ => raise Error ctx)
+  | _ => raise Error ctx
+End
+
+Definition update_current_stmt_def:
+  update_current_statement st ctx =
+  ctx with current_fc updated_by
+    (λfc. fc with current_stmt := st)
+End
+
+Definition return_expr_def:
+  return_expr v (StartExpr _) = ErrorExpr ∧
+  return_expr v (IfExpK k e1 e2) = IfExpK (return_expr v k) e1 e2  ∧
+  return_expr v (ArrayLitK vs k es) = ArrayLitK vs (return_expr v k) es ∧
+  return_expr v (SubscriptK1 k e) = SubscriptK1 (return_expr v k) e ∧
+  return_expr v (SubscriptK2 v k) = SubscriptK2 v (return_expr v k) ∧
+  return_expr v (AttributeK k id) = AttributeK (return_expr v k) id ∧
+  return_expr v (CompareK1 k cmp e) = CompareK1 (return_expr v k) cmp e ∧
+  return_expr v (CompareK2 v cmp k) = CompareK2 v cmp (return_expr v k) ∧
+  return_expr v (BinOpK1 k bop e) = BinOpK1 (return_expr v k) bop e ∧
+  return_expr v (BinOpK2 v bop k) = BinOpK2 v bop (return_expr v k) ∧
+  return_expr v (CallK id vs k es) = CallK id vs (return_expr v k) es ∧
+  return_expr v (LiftCall fn vs k) = LiftCall fn vs (return_expr v k) ∧
+  return_expr v (DoneExpr _) = ErrorExpr ∧
+  return_expr v ReturnExpr = DoneExpr v ∧
+  return_expr v ErrorExpr = ErrorExpr
+End
+
+Definition return_base_tgt_def:
+  return_base_tgt v (StartBaseTgt _) = NONE ∧
+  return_base_tgt v (SubscriptTargetK1 k e) =
+    OPTION_MAP (λk. SubscriptTargetK1 k e) (return_base_tgt v k) ∧
+  return_base_tgt v (SubscriptTargetK2 l s k) =
+    SOME (SubscriptTargetK2 l s (return_expr v k)) ∧
+  return_base_tgt v (AttributeTargetK k id) =
+    OPTION_MAP (λk. AttributeTargetK k id) (return_base_tgt v k) ∧
+  return_base_tgt v (LiftCallBaseTgt fn vs k) =
+    OPTION_MAP (λk. LiftCallBaseTgt fn vs k) (return_base_tgt v k) ∧
+  return_base_tgt _ _ = NONE
+End
+
+Definition return_tgt_def:
+  return_tgt v (StartTgt _) = ErrorTgt ∧
+  return_tgt v (TupleTargetK vs k as) =
+    TupleTargetK vs (return_tgt v k) as ∧
+  return_tgt v (BaseTargetK t) =
+    (case return_base_tgt v t of NONE => ErrorTgt
+        | SOME t => BaseTargetK t) ∧
+  return_tgt v (LiftCallTgt fn vs k) =
+    LiftCallTgt fn vs (return_tgt v k) ∧
+  return_tgt v (DoneTgt _) = ErrorTgt ∧
+  return_tgt v ErrorTgt = ErrorTgt
+End
+
+Definition return_def:
+  return v (ForK id typ k ss) = ForK id typ (return_expr v k) ss ∧
+  return v (IfK k s1 s2) = IfK (return_expr v k) s1 s2 ∧
+  return v (AssertK k s) = AssertK (return_expr v k) s ∧
+  return v (ReturnSomeK k) = ReturnSomeK (return_expr v k) ∧
+  return v (AssignK1 t e) = AssignK1 (return_tgt v t) e ∧
+  return v (AssignK2 a k) = AssignK2 a (return_expr v k) ∧
+  return v (AugAssignK id op k) = AugAssignK id op (return_expr v k) ∧
+  return v (AnnAssignK id typ k) = AnnAssignK id typ (return_expr v k) ∧
+  return v _ = ExceptionK Error
+End
+
+Definition pop_call_def:
+  pop_call v ctx =
+  case ctx.call_stack of fc::fcs =>
+    if IS_SOME fc.loop then
+      pop_call v (ctx with call_stack := fcs)
+    else
+      ctx with <|
+          current_fc := fc with current_stmt updated_by return v
+        ; call_stack := fcs
+        |>
+  | _ => raise (ExternalReturn v) ctx
+Termination
+  WF_REL_TAC`measure (λx. LENGTH (SND x).call_stack)` \\ rw[]
+End
+
+Definition set_stmt_def:
+  set_stmt k ctx =
+    ctx with current_fc updated_by (λfc. fc with current_stmt := k)
+End
+
+Definition exception_raised_def:
+  exception_raised ctx <=>
+  case ctx.current_fc.current_stmt of ExceptionK _ => T | _ => F
+End
+
+Definition push_loop_def:
+  push_loop id typ (v::vs) (s::ss) ctx =
+    ctx with <|
+      call_stack updated_by CONS ctx.current_fc
+    ; current_fc := <|
+        scopes := (FEMPTY |+ (id,v))::ctx.current_fc.scopes
+      ; current_stmt := (StartK s)
+      ; remaining_stmts := ss
+      ; loop := SOME <|
+          loop_var := id
+        ; remaining_values := vs
+        ; loop_first_stmt := s
+        ; loop_rest_stmts := ss
+        |>
+      |>
+    |> ∧
+  push_loop _ _ [] (_::_) ctx = set_stmt DoneK ctx ∧
+  push_loop _ _ _ _ ctx = raise Error ctx
+End
+
+Definition pop_loop_def:
+  pop_loop ctx =
+  case ctx.call_stack of
+     | [] => raise Error ctx
+     | fc::fcs => ctx with <| current_fc := fc; call_stack := fcs |>
+End
+
+Definition next_iteration_def:
+  next_iteration li ctx =
+  case li.remaining_values of [] => pop_loop ctx
+     | v::vs => ctx with current_fc updated_by (λfc.
+        fc with <| scopes updated_by CONS (FEMPTY |+ (li.loop_var, v))
+                 ; current_stmt := StartK li.loop_first_stmt
+                 ; remaining_stmts := li.loop_rest_stmts
+                 ; loop := SOME (li with remaining_values := vs) |>)
+End
+
+Definition continue_loop_def:
+  continue_loop ctx =
+  case ctx.current_fc.loop of SOME li => (
+    let ctx = pop_scope ctx in
+      if exception_raised ctx then ctx else
+        next_iteration li ctx
+  ) | _ => raise Error ctx
+End
+
+Definition break_loop_def:
+  break_loop ctx =
+  case ctx.current_fc.loop of SOME li => (
+    let ctx = pop_scope ctx in
+      if exception_raised ctx then ctx else
+        pop_loop ctx
+  ) | _ => raise Error ctx
+End
+
+Definition next_stmt_def:
+  next_stmt ctx =
+  case ctx.current_fc.remaining_stmts of s::ss =>
+    ctx with current_fc updated_by (λfc.
+      fc with <| current_stmt := StartK s
+               ; remaining_stmts := ss |>)
+  | _ => (case ctx.current_fc.loop
+            of NONE => pop_call VoidV ctx
+             | SOME li => next_iteration li ctx)
+End
+
+Definition step_stmt_def:
+  step_stmt ctx =
+  let fc = ctx.current_fc in
+  (case fc.current_stmt of
+      | StartK Pass => set_stmt DoneK ctx
+      | StartK Continue => continue_loop ctx
+      | StartK Break => break_loop ctx
+      | StartK (Raise s) => raise (RaiseException s) ctx
+      | StartK (Assert e s) => set_stmt (AssertK (StartExpr e) s) ctx
+      | StartK (Return NONE) => pop_call VoidV ctx
+      | StartK (Return (SOME e)) =>
+          set_stmt (ReturnSomeK (StartExpr e)) ctx
+      | StartK (AnnAssign id typ e) =>
+          set_stmt (AnnAssignK id typ (StartExpr e)) ctx
+      | StartK (AugAssign id bop e) =>
+          set_stmt (AugAssignK id bop (StartExpr e)) ctx
+      | StartK (Assign tgt e) =>
+          set_stmt (AssignK1 (StartTgt tgt) e) ctx
+      | StartK (If e s1 s2) =>
+          set_stmt (IfK (StartExpr e) s1 s2) ctx
+      | StartK (For id typ e s) =>
+          set_stmt (ForK id typ (StartExpr e) s) ctx
+      | IfK (DoneExpr (BoolV b)) s1 s2 => (
+          case (if b then s1 else s2) of s::ss =>
+            ctx with current_fc := fc with
+              <| current_stmt := StartK s
+               ; remaining_stmts updated_by (λx. ss ++ x) |>
+          | _ => raise Error ctx)
+      | IfK (DoneExpr _) _ _ => raise Error ctx
+      | IfK ErrorExpr _ _ => raise Error ctx
+      | IfK ReturnExpr _ _ => raise Error ctx
+      | IfK (LiftCall fn vs k) s1 s2 =>
+          push_call fn vs
+            (set_stmt (IfK k s1 s2) ctx)
+      | IfK k s1 s2 =>
+          set_stmt
+            (IfK (step_expr ctx.globals fc.scopes k) s1 s2) ctx
+      | AssertK (DoneExpr (BoolV b)) s => (
+          if b then set_stmt DoneK ctx
+          else raise (AssertException s) ctx)
+      | AssertK (DoneExpr _) _ => raise Error ctx
+      | AssertK ErrorExpr _ => raise Error ctx
+      | AssertK ReturnExpr _ => raise Error ctx
+      | AssertK (LiftCall fn vs k) s =>
+          push_call fn vs
+            (set_stmt (AssertK k s) ctx)
+      | AssertK k s =>
+          set_stmt (AssertK (step_expr ctx.globals fc.scopes k) s) ctx
+      | ReturnSomeK (DoneExpr v) => pop_call v ctx
+      | ReturnSomeK ErrorExpr => raise Error ctx
+      | ReturnSomeK ReturnExpr => raise Error ctx
+      | ReturnSomeK (LiftCall fn vs k) =>
+          push_call fn vs
+            (set_stmt (ReturnSomeK k) ctx)
+      | ReturnSomeK k =>
+          set_stmt
+            (ReturnSomeK (step_expr ctx.globals fc.scopes k)) ctx
+      | AssignK1 (DoneTgt av) e =>
+          set_stmt (AssignK2 av (StartExpr e)) ctx
+      | AssignK1 ErrorTgt e => raise Error ctx
+      | AssignK1 (LiftCallTgt fn vs tk) e =>
+          push_call fn vs
+            (set_stmt (AssignK1 tk e) ctx)
+      | AssignK1 tk e =>
+          set_stmt
+            (AssignK1 (step_target ctx.globals fc.scopes tk) e) ctx
+      | AssignK2 tv (DoneExpr v) =>
+          set_stmt DoneK (assign_target tv v ctx)
+      | AssignK2 tv ErrorExpr => raise Error ctx
+      | AssignK2 tv ReturnExpr => raise Error ctx
+      | AssignK2 tv (LiftCall fn vs k) =>
+          push_call fn vs
+            (set_stmt (AssignK2 tv k) ctx)
+      | AssignK2 tv k =>
+          set_stmt
+            (AssignK2 tv (step_expr ctx.globals fc.scopes k)) ctx
+      | AugAssignK id bop (DoneExpr v2) =>
+        (case lookup_scopes id fc.scopes
+           of NONE => raise Error ctx
+            | SOME v1 =>
+              (case evaluate_binop bop v1 v2
+                 of DoneExpr v => set_stmt DoneK (set_variable id v ctx)
+                  | _ => raise Error ctx))
+      | AugAssignK id bop ErrorExpr => raise Error ctx
+      | AugAssignK id bop ReturnExpr => raise Error ctx
+      | AugAssignK id bop (LiftCall fn vs k) =>
+          push_call fn vs
+            (set_stmt (AugAssignK id bop k) ctx)
+      | AugAssignK id bop k =>
+          set_stmt
+            (AugAssignK id bop (step_expr ctx.globals fc.scopes k)) ctx
+      | AnnAssignK id typ (DoneExpr v) => (
+          let ctx = new_variable id typ ctx in
+            if exception_raised ctx then ctx else
+              set_stmt DoneK (set_variable id v ctx))
+      | AnnAssignK id typ ErrorExpr => raise Error ctx
+      | AnnAssignK id typ ReturnExpr => raise Error ctx
+      | AnnAssignK id typ (LiftCall fn vs k) =>
+          push_call fn vs
+            (set_stmt (AnnAssignK id typ k) ctx)
+      | AnnAssignK id typ k =>
+          set_stmt (AnnAssignK id typ (step_expr ctx.globals fc.scopes k)) ctx
+      | ExceptionK err => ctx
+      | DoneK => next_stmt ctx
+      | ForK id typ (DoneExpr (ArrayV [])) (st::ss) =>
+          set_stmt DoneK ctx
+      | ForK id typ (DoneExpr (ArrayV vs)) ss =>
+          push_loop id typ vs ss ctx
+      | ForK id typ (DoneExpr _) _ => raise Error ctx
+      | ForK id typ ErrorExpr _ => raise Error ctx
+      | ForK id typ ReturnExpr _ => raise Error ctx
+      | ForK id typ (LiftCall fn vs k) ss =>
+          push_call fn vs
+            (set_stmt (ForK id typ k ss) ctx)
+      | ForK id typ k ss =>
+          set_stmt (ForK id typ (step_expr ctx.globals fc.scopes k) ss) ctx)
 End
 
 Definition external_call_def:
   external_call n name args ts =
-  let gbs = initial_globals ts in
   case lookup_external_function name ts of
     SOME (params, _, body) =>
     (case bind_arguments params args of
        SOME env =>
        (let fc = initial_function_context env body in
-        let ctx = initial_execution_context gbs fc in
-        let ctx = execute_stmts n body ctx in
-          ctx.raised)
-     | _ => SOME Error)
-  | _ => SOME Error
+        let ctx = initial_execution_context ts fc in
+        let ctx = FUNPOW step_stmt n ctx in
+        (case ctx.current_fc.current_stmt
+           of ExceptionK (ExternalReturn v) => SOME v
+            | _ => NONE))
+     | _ => NONE)
+  | _ => NONE
 End
 
 val () = export_theory();
